Start working on proofs for DB code.

store/impl.v
@@ -4,6 +4,7 @@ From stdpp Require Import namespaces.
 From iris.algebra Require Import agree auth csum gset gmap excl frac.
 From iris.algebra Require Import max_prefix_list.
 From iris.heap_lang Require Import notation proofmode.
+From iris.heap_lang.lib Require Import lock ticket_lock.
 From cryptis Require Import lib version term cryptis primitives tactics.
 From cryptis Require Import role session pk_auth pk_dh.
 
@@ -87,6 +88,51 @@ Definition load : val := λ: "c" "cs",
 End Client.
 
 End Client.
+
+Module DB.
+
+Definition new : val := λ: <>,
+  let: "kvs" := ref [] in
+  let: "lock" := newlock #() in
+  ("kvs", "lock").
+
+Definition find : val := λ: "kvs" "k",
+  let: "res" := find_list (λ: "kv", eq_term (Fst "kv") "k") "kvs" in
+  match: "res" with
+    SOME "res" => SOME (Snd "res")
+  | NONE => NONE
+  end.
+
+Definition with_locked_db : val := λ: "db" "f",
+  let: "kvs" := Fst "db" in
+  let: "lock" := Snd "db" in
+  acquire "lock";;
+  let: "res" := "f" "kvs" in
+  release "lock";;
+  "res".
+
+Definition set : val := λ: "db" "k" "v",
+  with_locked_db "db" (λ: "kvs",
+      "kvs" <- ("k", "v") :: !"kvs";;
+      #()
+  ).
+
+Definition get : val := λ: "db" "k",
+  with_locked_db "db" (λ: "kvs",
+      match: find !"kvs" "k" with
+        SOME "res" => "res"
+      | NONE => #() (* Error *)
+      end).
+
+Definition create : val := λ: "db" "k" "v",
+  with_locked_db "db" (λ: "kvs",
+    match: find !"kvs" "k" with
+      SOME <> => #false
+    | NONE => "kvs" <- ("k", "v") :: !"kvs";; #true
+    end
+  ).
+
+End DB.
 
 Record sst := {
   sst_ts   : loc;
