store/db_proofs.v
@@ -1,0 +1,237 @@
+From stdpp Require Import base countable gmap.
+From mathcomp Require Import ssreflect.
+From stdpp Require Import namespaces.
+From iris.algebra Require Import agree auth csum gset gmap excl frac.
+From iris.algebra Require Import max_prefix_list.
+From iris.heap_lang Require Import notation proofmode.
+From iris.heap_lang.lib Require Import lock ticket_lock.
+From cryptis Require Import lib version term cryptis primitives tactics.
+From cryptis.store Require Import impl shared.
+
+Set Implicit Arguments.
+Unset Strict Implicit.
+Unset Printing Implicit Defensive.
+
+Definition dbUR : ucmra :=
+  authUR (gmapUR term (exclR termO)).
+
+Class dbGpreS Σ :=  DbGpreS {
+  dbGpreS_tlock : tlockG Σ;
+  dbGpreS_db : inG Σ dbUR;
+}.
+
+Local Existing Instance dbGpreS_tlock.
+Local Existing Instance dbGpreS_db.
+
+Class dbGS Σ := DbGS {
+  db_inG : dbGpreS Σ;
+}.
+
+Local Existing Instance db_inG.
+
+Section Verif.
+
+Context `{!cryptisGS Σ, !heapGS Σ, !dbGS Σ}.
+Notation iProp := (iProp Σ).
+
+Implicit Types (γ : gname) (l : loc) (t : term) (v : val).
+Implicit Types (kvs : list (term * term)) (db : gmap term term).
+
+Definition is_alist kvs db : Prop :=
+  ∀ k, db !! k = snd <$> find (λ p, bool_decide (p.1 = k)) kvs.
+
+Definition stores_db l db : iProp :=
+  ∃ kvs, l ↦ repr kvs ∗ ⌜is_alist kvs db⌝.
+
+Definition db_auth db : dbUR :=
+  ● (Excl <$> db).
+
+Definition db_frag db : dbUR :=
+  ◯ (Excl <$> db).
+
+Lemma valid_db_auth db : ✓ db_auth db.
+Proof.
+apply/auth_auth_valid => k; rewrite lookup_fmap; by case: (db !! k).
+Qed.
+
+Lemma valid_db_frag db : ✓ db_frag db.
+Proof.
+apply/auth_frag_valid => k; rewrite lookup_fmap; by case: (db !! k).
+Qed.
+
+Hint Resolve valid_db_auth : core.
+
+Lemma db_auth_db_frag_valid db1 db2 :
+  ✓ (db_auth db1 ⋅ db_frag db2) →
+  ∀ t1 t2, db2 !! t1 = Some t2 -> db1 !! t1 = Some t2.
+Proof.
+rewrite /db_auth /db_frag => /auth_both_valid_discrete [incl_12 valid_1] t1 t2.
+move: incl_12; rewrite lookup_included; move/(_ t1).
+rewrite !lookup_fmap => incl_12 db2_t1.
+rewrite db2_t1 /= in incl_12.
+case db1_t1: (db1 !! t1) => [t2'|] /= in incl_12 *.
+- by move/Excl_included/(leibniz_equiv _ _): incl_12 => ->.
+- by case/option_included: incl_12 => // - [] ? [] ? [] ? [] ?.
+Qed.
+
+Lemma db_auth_db_frag1_valid db t1 t2 :
+  ✓ (db_auth db ⋅ db_frag {[t1 := t2]}) →
+  db !! t1 = Some t2.
+Proof.
+move=> valid_12; apply: (db_auth_db_frag_valid valid_12).
+by rewrite lookup_singleton.
+Qed.
+
+Lemma db_auth_db_frag_update db t1 t2 t2' :
+  db_auth db ⋅ db_frag {[t1 := t2]} ~~>
+  db_auth (<[t1 := t2']> db) ⋅ db_frag {[t1 := t2']}.
+Proof.
+apply/auth_update; rewrite fmap_insert !map_fmap_singleton.
+apply: singleton_local_update_any => x _.
+by apply: exclusive_local_update.
+Qed.
+
+Definition db_res γ l : iProp :=
+  ∃ db, stores_db l db ∗ own γ (db_auth db).
+
+Definition is_db v : iProp :=
+  ∃ l vlock γkvs γlock,
+    ⌜v = (#l, vlock)%V⌝ ∗
+    meta l (nroot.@"kvs") γkvs ∗
+    meta l (nroot.@"lock") γlock ∗
+    is_lock γlock vlock (db_res γkvs l).
+
+Global Instance is_db_persistent v : Persistent (is_db v).
+Proof. apply _. Qed.
+
+Lemma wp_db_new :
+  {{{ True }}}
+    DB.new #()
+  {{{ v, RET v; is_db v }}}.
+Proof.
+iIntros "%Φ _ Hpost"; wp_lam; wp_pures.
+wp_bind (ref _)%E; iApply wp_alloc => //.
+iIntros "!> %l [Hl meta]".
+rewrite (meta_token_difference _ (↑(nroot.@"kvs")) _) //.
+iDestruct "meta" as "[meta_kvs meta]".
+iMod (own_alloc (db_auth ∅)) as "[%γkvs own_γkvs]" => //.
+iMod (meta_set _ _ γkvs (nroot.@"kvs") with "meta_kvs") as "#meta_kvs" => //.
+wp_pures; wp_bind (newlock _).
+iApply (newlock_spec (db_res γkvs l) with "[Hl own_γkvs]").
+{ iExists ∅. iFrame. iExists [].
+  rewrite /=. rewrite repr_list_unseal /=. iFrame.
+  by iPureIntro => k; rewrite lookup_empty. }
+iIntros "!> %vlock %γlock #lock".
+iMod (meta_set _ _ γlock (nroot.@"lock") with "meta") as "#meta_lock".
+{ solve_ndisj. }
+wp_pures. iApply "Hpost". iExists l, vlock, γkvs, γlock. eauto.
+Qed.
+
+Lemma wp_find kvs db t :
+  is_alist kvs db →
+  {{{ True }}}
+    DB.find (repr kvs) t
+  {{{ RET (repr (db !! t)); True }}}.
+Proof.
+iIntros "%kvs_db %Φ _ Hpost"; wp_lam; wp_pures.
+wp_bind (find_list _ _).
+iApply (wp_find_list (λ x, bool_decide (x.1 = t)) _ kvs) => //.
+{ move=> [k t']; iIntros "%Φ' _ Hpost".
+  wp_pures. iApply wp_eq_term. by iApply "Hpost". }
+iIntros "!> _"; rewrite kvs_db.
+by case: find => [[k' t']|] /=; wp_pures; iApply "Hpost".
+Qed.
+
+Lemma wp_with_locked_db v Φ (f : val) :
+  (∀ γkvs l vlock,
+      ⌜v = (#l, vlock)%V⌝ -∗
+      meta l (nroot.@"kvs") γkvs -∗
+      db_res γkvs l -∗
+      WP f #l {{ res, Φ res ∗ db_res γkvs l }}) -∗
+  is_db v -∗
+  WP DB.with_locked_db v f {{ res, Φ res }}.
+Proof.
+iIntros "wp_f (%l & %vlock & %γkvs & %γloc & -> & #m_kvs & #m_lock & #lock)".
+wp_lam; wp_pures.
+wp_bind (acquire _); iApply (acquire_spec with "lock").
+iIntros "!> (locked & db_res)".
+wp_pures; wp_bind (f _).
+iPoseProof ("wp_f" with "[//] m_kvs db_res") as "wp_f".
+iApply (wp_wand with "wp_f").
+iIntros "%res [post db_res]".
+wp_pures; wp_bind (release _); iApply (release_spec with "[locked db_res]").
+{ iFrame. iSplitR; eauto. }
+iIntros "!> _"; wp_pures; eauto.
+Qed.
+
+Definition db_mapsto v t1 t2 : iProp :=
+  ∃ l vlock γkvs,
+    ⌜v = (#l, vlock)%V⌝ ∗
+    meta l (nroot.@"kvs") γkvs ∗
+    own γkvs (db_frag {[t1 := t2]}).
+
+Lemma db_mapsto_inv l v γkvs t1 t2 :
+  db_mapsto (#l, v)%V t1 t2 -∗
+  meta l (nroot.@"kvs") γkvs -∗
+  own γkvs (db_frag {[t1 := t2]}).
+Proof.
+iIntros "(%l' & %v' & %γkvs' & %E & #meta' & own) #meta".
+case: E => <- _ {l' v'}.
+now iPoseProof (meta_agree with "meta meta'") as "<-".
+Qed.
+
+Lemma is_alist_cons kvs db k t :
+  is_alist kvs db ->
+  is_alist ((k, t) :: kvs) (<[k := t]>db).
+Proof.
+move=> kvs_db k' /=; case: bool_decide_reflect => [<-|ne].
+- by rewrite lookup_insert.
+- by rewrite lookup_insert_ne.
+Qed.
+
+Lemma wp_set v t1 t2 t2' :
+  {{{ is_db v ∗ db_mapsto v t1 t2 }}}
+    DB.set v t1 t2'
+  {{{ RET #(); db_mapsto v t1 t2' }}}.
+Proof.
+iIntros "%Φ [#vP t1_t2] Hpost".
+wp_lam; wp_pures; iApply (wp_with_locked_db with "[t1_t2 Hpost] vP").
+iIntros "%γkvs %l %vlock -> #m_kvs lP".
+iPoseProof (db_mapsto_inv with "t1_t2 m_kvs") as "t1_t2".
+iDestruct "lP" as "(%db & (%kvs & l_kvs & %kvs_db) & dbP)".
+iPoseProof (own_valid_2 with "dbP t1_t2") as "%valid_12".
+have {valid_12} db_t1 := db_auth_db_frag1_valid valid_12.
+wp_pures. wp_load. wp_pures. change (t1, t2')%V with (repr (t1, t2')).
+(* FIXME: The wp_cons tactic cannot proceed here because it undoes the previous
+   change, which brings the goal to a shape where the tac_wp_cons lemma does not
+   apply. *)
+wp_bind (_ :: _)%E. iApply (wp_cons _ (t1, t2') kvs). wp_store.
+iMod (own_update_2 with "dbP t1_t2") as "Hown".
+  exact: (db_auth_db_frag_update t2').
+iDestruct "Hown" as "[dbP t1_t2]".
+iModIntro. iSplitL "Hpost t1_t2".
+- iApply "Hpost". iExists l, vlock, γkvs; eauto.
+- iExists _; iFrame. iExists _. iFrame. iPureIntro.
+  exact: is_alist_cons.
+Qed.
+
+Lemma wp_get v t1 t2 :
+  {{{ is_db v ∗ db_mapsto v t1 t2 }}}
+    DB.get v t1
+  {{{ RET (repr t2); db_mapsto v t1 t2 }}}.
+Proof.
+iIntros "%Φ [#vP t1_t2] Hpost".
+wp_lam; wp_pures; iApply (wp_with_locked_db with "[t1_t2 Hpost] vP").
+iIntros "%γkvs %l %vlock -> #m_kvs lP".
+iPoseProof (db_mapsto_inv with "t1_t2 m_kvs") as "t1_t2".
+iDestruct "lP" as "(%db & (%kvs & l_kvs & %kvs_db) & dbP)".
+iPoseProof (own_valid_2 with "dbP t1_t2") as "%valid_12".
+have {valid_12} db_t1 := db_auth_db_frag1_valid valid_12.
+wp_pures. wp_load. wp_bind (DB.find _ _)%E. iApply wp_find; eauto.
+iIntros "!> _". rewrite db_t1. wp_pures. iModIntro.
+iSplitL "Hpost t1_t2".
+- iApply "Hpost". iExists l, vlock, γkvs. eauto.
+- iExists _; iFrame. iExists _. iFrame. eauto.
+Qed.
+
+End Verif.
